

CFG Normal Forms

CNF Form

Removal of Left Recursion

GNF Form

Normal Forms

- A grammar is said to be in a Normal Form when every production of a grammar has specific form
- This makes it convenient to design algorithms for working with CFGs

Normal Forms for CFG

- CNF, Chomsky Normal Form
- GNF, Greibach Normal Form

CNF, Chomsky Normal Form

- A grammar is said to be in Chomsky Normal form (i.e. CNF) if every production rule of the grammar is of the form:
 $A \rightarrow BC$ or $A \rightarrow a$
- where A, B, C are in V and a is in T

Conversion to CNF

Step 1: Simplify the grammar G by **eliminating null productions, useless productions and unit productions**

Step 2: Add to the solution, the productions which are already in CNF

Step 3: For the productions, not in CNF:-

- a) **Replace the terminals by some variables**
- b) **limit the number of variables on RHS to 2**

CNF, Chomsky Normal Form-Example 1

- Consider a CFG with following productions:

$S \rightarrow aB \mid bA$

$A \rightarrow a \mid aS \mid bAA$

$B \rightarrow b \mid bS \mid aBB$

CNF, Chomsky Normal Form-Example 1

- Consider a CFG with following productions:

$S \rightarrow aB \mid bA$

$A \rightarrow a \mid aS \mid bAA$

$B \rightarrow b \mid bS \mid aBB$

Solution-

Introduce new non-terminals C_a and C_b and production

$C_a \rightarrow a$ and $C_b \rightarrow b$, we get:-

$S \rightarrow C_a B \mid C_b A$

$A \rightarrow a \mid C_a S \mid C_b AA$

$B \rightarrow b \mid C_b S \mid C_a BB$

CNF, Chomsky Normal Form-Example 1

$S \rightarrow C_a B \mid C_b A$

$A \rightarrow a \mid C_a S \mid C_b AA$

$B \rightarrow b \mid C_b S \mid C_a BB$

$C_a \rightarrow a$

$C_b \rightarrow b$

Introduce D_1 and D_2 as two new non-terminals and productions

$D_1 \rightarrow AA$ and $D_2 \rightarrow BB$

We get,

$S \rightarrow C_a B \mid C_b A$

$A \rightarrow a \mid C_a S \mid C_b D_1$

$B \rightarrow b \mid C_b S \mid C_a D_2$

$C_a \rightarrow a$

$C_b \rightarrow b$

$D_1 \rightarrow AA$

$D_2 \rightarrow BB$

The grammar is in CNF

CNF, Chomsky Normal Form-Example 2

Consider a CFG with the following productions:

$S \rightarrow aSa \mid bSb \mid ab$

CNF, Chomsky Normal Form-Example 2

Consider a CFG with the following productions:

$$S \rightarrow aSa \mid bSb \mid ab$$

Introducing new non-terminals C_a and C_b , we get

$$S \rightarrow C_a S C_a \mid C_b S C_b \mid C_a C_b$$
$$C_a \rightarrow a$$
$$C_b \rightarrow b$$

Introducing D_1 and D_2 , we get

$$S \rightarrow C_a D_1 \mid C_b D_2 \mid C_a C_b$$
$$C_a \rightarrow a$$
$$C_b \rightarrow b$$
$$D_1 \rightarrow S C_a$$
$$D_2 \rightarrow S C_b$$

The grammar is in CNF

CNF, Chomsky Normal Form-Example 3

Consider a CFG with the following productions:

$S \rightarrow aSb \mid aA \mid bB \mid a \mid b$

$A \rightarrow aA \mid a$

$B \rightarrow bB \mid b$

CNF, Chomsky Normal Form-Example 3

Consider a CFG with the following productions:

$$S \rightarrow aSb \mid aA \mid bB \mid a \mid b$$
$$A \rightarrow aA \mid a$$
$$B \rightarrow bB \mid b$$

CNF, Chomsky Normal Form-Example 3

Consider a CFG with the following productions:

$$S \rightarrow aSb \mid aA \mid bB \mid a \mid b$$
$$A \rightarrow aA \mid a$$
$$B \rightarrow bB \mid b$$

Introducing new non-terminals C_a and C_b , we get

$$S \rightarrow C_a S C_b \mid C_a A \mid C_b B \mid a \mid b$$
$$A \rightarrow C_a A \mid a$$
$$B \rightarrow C_b B \mid b$$
$$C_a \rightarrow a$$
$$C_b \rightarrow b$$

Introducing D_1 , we get

$$S \rightarrow C_a D_1 \mid C_a A \mid C_b B \mid a \mid b$$
$$A \rightarrow C_a A \mid a$$
$$B \rightarrow C_b B \mid b$$
$$C_a \rightarrow a$$
$$C_b \rightarrow b$$
$$D_1 \rightarrow S C_b$$

The grammar is in CNF

Elimination of Left Recursion

- If a grammar contains a pair of productions of the form $A \rightarrow A\alpha \mid \beta$
- then the grammar is left recursive grammar
- Left recursive grammar , if used for specification of the language then the top down parser may enter into the infinite loop during the parsing process on some erroneous input.

Elimination of Left Recursion

Left recursion can be eliminated from the grammar by the following rule-
 $G=(V,T,P,S)$

For Production P:-

$A \rightarrow A\alpha_1 | A\alpha_2 | \dots | A\alpha_m | \beta_1 | \beta_2 | \dots | \beta_n$

β does not start with A

Replace by P1-

$A \rightarrow \beta_1 Z | \beta_2 Z | \dots | \beta_n | \beta_1 | \beta_2 | \dots | \beta_n$

$Z \rightarrow \alpha_1 Z | \alpha_2 Z | \dots | \alpha_m Z | \alpha_1 | \alpha_2 | \dots | \alpha_m$

OR

$A \rightarrow \beta_1 Z | \beta_2 Z | \dots | \beta_n Z$

$Z \rightarrow \alpha_1 Z | \alpha_2 Z | \dots | \alpha_m Z | \epsilon$

Without Null
Approach

With Null Approach

New Grammar $G1=(V \cup \{Z\}, T, P1, S)$

Elimination of Left Recursion-Example 1

Consider the following grammar:

$S \rightarrow aBDh$

$B \rightarrow Bb \mid c$

$D \rightarrow EF$

$E \rightarrow g \mid \epsilon$

$F \rightarrow f \mid \epsilon$

Elimination of Left Recursion-Example 1

Consider the following grammar:

$S \rightarrow aBDh$

$B \rightarrow Bb \mid c$

$D \rightarrow EF$

$E \rightarrow g \mid \epsilon$

$F \rightarrow f \mid \epsilon$

The grammar is left recursive due to production

$B \rightarrow Bb \mid c$

To eliminate the left recursion from the grammar,

Replace this pair of production by:-

$B \rightarrow cZ$

$Z \rightarrow bZ \mid \epsilon$

Thus, Final grammar is :-

$S \rightarrow aBDh$

$B \rightarrow cZ$

$Z \rightarrow bZ \mid \epsilon$

$D \rightarrow EF$

$E \rightarrow g \mid \epsilon$

$F \rightarrow f \mid \epsilon$

With Null Approach

Elimination of Left Recursion-Example 2

Consider the following grammar:

$S \rightarrow A$

$A \rightarrow Ad | Ae | aB | aC$

$B \rightarrow bBC | f$

$C \rightarrow g$

Elimination of Left Recursion-Example 2

Consider the following grammar:

$S \rightarrow A$

$A \rightarrow Ad | Ae | aB | aC$

$B \rightarrow bBC | f$

$C \rightarrow g$

The grammar is left recursive due to production

$A \rightarrow Ad | Ae | aB | aC$

To eliminate the left recursion from the grammar,

Replace this pair of production by:-

$A \rightarrow aBZ | aCZ$

$Z \rightarrow dZ | eZ | \epsilon$

Thus, Final grammar is :-

$S \rightarrow A$

$A \rightarrow aBZ | aCZ$

$Z \rightarrow dZ | eZ | \epsilon$

$B \rightarrow bBC | f$

$C \rightarrow g$

With Null Approach

Elimination of Left Recursion-Example 3

Consider the following grammar:

$A \rightarrow aBD \mid bDB \mid c$

$A \rightarrow AB \mid AD$

Remove left recursion

Elimination of Left Recursion-Example 3

Consider the following grammar:

$A \rightarrow aBD \mid bDB \mid c$

$A \rightarrow AB \mid AD$

Remove left recursion

To eliminate the left recursion from the grammar,

Replace :-

$A \rightarrow AB \mid AD$

By this pair of production by:-

$A \rightarrow aBDZ \mid bDBZ \mid cZ$

$Z \rightarrow BZ \mid DZ \mid \epsilon$

GNF

GNF, Greibach Normal Form

- A grammar is said to be in **Greibach** Normal form (i.e. GNF) if every production rule of the grammar is of the form:

$$A \rightarrow a\alpha$$

- where A is the non terminal, a is the terminal and α is a string of non-terminals (possibly empty)
- α belongs to V^*

GNF, Greibach Normal Form

- Divide the production of Grammar G into left recursive and non-left recursive production
- Then eliminate left recursion to get GNF

Conversion to GNF

Step 1: Simplify the grammar G by **eliminating null productions, useless productions and unit productions**

Step 2: Add to the solution, the productions which are already in GNF

Step 3: For the productions, not in GNF:-

a) **Use Substitution Rule**

$A \rightarrow B\alpha$

$B \rightarrow \beta_1 \mid \beta_2 \mid \dots \mid \beta_n$

then we can write A as

$A \rightarrow \beta_1\alpha \mid \beta_2\alpha \mid \dots \mid \beta_n\alpha$

b) **Remove left recursion , Use without epsilon approach**

GNF, Greibach Normal Form-Example 1

Consider a CFG with the following productions, Convert to GNF:

$S \rightarrow aSa \mid bSb \mid ab$

For GNF-

$A \rightarrow a\alpha$

where A is the non terminal, a is the terminal and α is a string of non-terminals(possibly empty)

GNF, Greibach Normal Form-Example 1

Consider a CFG with the following productions, Convert to GNF :

$S \rightarrow aSa \mid bSb \mid ab$

Soln:

$S \rightarrow aSA \mid bSB \mid aB$

$A \rightarrow a$

$B \rightarrow b$

The grammar is in GNF

For GNF-

$A \rightarrow a\alpha$

where A is the non terminal, a is the terminal and α is a string of **non-terminals(possibly empty)**

Simple Variable Usage

GNF, Greibach Normal Form-Example 2

- Consider a CFG with the following productions, Convert to GNF :

$S \rightarrow XY \mid XW$

$X \rightarrow YZ \mid a$

$Z \rightarrow c$

$Y \rightarrow WZ \mid b$

$W \rightarrow d$

For GNF-

$A \rightarrow a\alpha$

where A is the non terminal, a is the terminal and α is a string of **non-terminals(possibly empty)**

Use Substitution Rule

GNF, Greibach Normal Form-Example 2

- Consider a CFG with the following productions, Convert to GNF :

$S \rightarrow XY \mid XW$

$X \rightarrow YZ \mid a$

$Z \rightarrow c$

$Y \rightarrow WZ \mid b$

$W \rightarrow d$

- Substitute W value in Y production

$Y \rightarrow WZ \mid b$, rewritten as-

$Y \rightarrow dZ \mid b$

- Substitute Y value in X production

$X \rightarrow YZ \mid a$, rewritten as-

$X \rightarrow dZZ \mid bZ \mid a$

- Substitute X value in S production

$S \rightarrow XY \mid XW$, rewritten as-

$S \rightarrow dZZY \mid bZY \mid aY \mid dZZW \mid bZW \mid aW$

- Final productions are-

$S \rightarrow dZZY \mid bZY \mid aY \mid dZZW \mid bZW \mid aW$

$X \rightarrow dZZ \mid bZ \mid a$

$Y \rightarrow dZ \mid b$

$W \rightarrow d$

$Z \rightarrow c$

GNF, Greibach Normal Form-Example 3

Consider a CFG with the following productions, Convert to GNF :

$S \rightarrow AA \mid 0$

$A \rightarrow SS \mid 1$

GNF, Greibach Normal Form-Example 3

Consider a CFG with the following productions, Convert to GNF :

$S \rightarrow AA \mid 0$

$A \rightarrow SS \mid 1$

GNF, Greibach Normal Form-Example 3

Consider a CFG with the following productions, Convert to GNF :

$S \rightarrow AA \mid 0$

$A \rightarrow SS \mid 1$

Substitute first S in production of A

$A \rightarrow SS \mid 1$

$A \rightarrow AAS \mid OS \mid 1$

Substitution Rule

So left recursion is there

To eliminate Left recursion-

$A \rightarrow OSZ \mid 1Z \mid OS \mid 1$

GNF Form

$Z \rightarrow ASZ \mid AS$

New Productions are:

$S \rightarrow AA \mid 0$

$A \rightarrow OSZ \mid 1Z \mid OS \mid 1$

Removal of Recursion

$Z \rightarrow ASZ \mid AS$

Now substitute the Value of A in S production

$S \rightarrow OSZA \mid 1ZA \mid OSA \mid 1A \mid 0$ GNF Form

$A \rightarrow OSZ \mid 1Z \mid OS \mid 1$ GNF Form

$Z \rightarrow ASZ \mid AS$

Substitution Rule

Now substitute the Value of A in Z production

$S \rightarrow OSZA \mid 1ZA \mid OSA \mid 1A \mid 0$ GNF Form

$A \rightarrow OSZ \mid 1Z \mid OS \mid 1$ GNF Form

$Z \rightarrow OSZSZ \mid 1ZSZ \mid OSSZ \mid 1SZ$

$OSZS \mid 1ZS \mid OSS \mid 1S$ GNF Form

Substitution Rule

GNF, Greibach Normal Form-Example 4

Convert the following grammar into GNF

$$E \rightarrow E+T \mid T$$
$$T \rightarrow T * F \mid F$$
$$F \rightarrow (E) \mid a$$

GNF, Greibach Normal Form-Example 4

Convert the following grammar into GNF

$$E \rightarrow E+T \mid T$$
$$T \rightarrow T * F \mid F$$
$$F \rightarrow (E) \mid a$$

Substitution Rule-

$$E \rightarrow E+T \mid T * F \mid F \text{ or } E \rightarrow E+T \mid T * F \mid (E) \mid a$$
$$T \rightarrow T * F \mid (E) \mid a$$
$$F \rightarrow (E) \mid a$$

Step 1: Remove unit productions

$$E \rightarrow T$$
$$T \rightarrow F$$

After removal of unit productions, we get

$$E \rightarrow E+T \mid T * F \mid (E) \mid a$$
$$T \rightarrow T * F \mid (E) \mid a$$
$$F \rightarrow (E) \mid a$$

GNF, Greibach Normal Form-Example 4

Step 2: Replace terminals of the productions which are not in GNF form by variables

$$E \rightarrow E+T \mid T^*F \mid (E) \mid a$$
$$T \rightarrow T^*F \mid (E) \mid a$$
$$F \rightarrow (E) \mid a$$

Introduce

$$A_1 \rightarrow +$$
$$A_2 \rightarrow *$$
$$A_3 \rightarrow)$$

The resulting Productions are-

$$E \rightarrow EA_1T \mid TA_2F \mid (EA_3 \mid a$$
$$T \rightarrow TA_2F \mid (EA_3 \mid a$$
$$F \rightarrow (EA_3 \mid a$$

Now all F productions are in GNF form

GNF, Greibach Normal Form-Example 4

Step 3: Remove Left Recursion for T

$E \rightarrow EA_1T \mid TA_2F \mid (EA_3 \mid a$

$T \rightarrow TA_2F \mid (EA_3 \mid a$

$F \rightarrow (EA_3 \mid a$

Left Recursion Removal-for T

Replace $T \rightarrow TA_2F \mid (EA_3 \mid a$ by

$T \rightarrow (EA_3Z_1 \mid aZ_1 \mid (EA_3 \mid a$

$Z_1 \rightarrow A_2FZ_1 \mid A_2F$

Substituting, we get

$A_2 \rightarrow ^*$

$T \rightarrow (EA_3Z_1 \mid aZ_1 \mid (EA_3 \mid a$

$Z_1 \rightarrow ^*FZ_1 \mid ^*F$

So Productions are

$E \rightarrow EA_1T \mid TA_2F \mid (EA_3 \mid a$

$T \rightarrow (EA_3Z_1 \mid aZ_1 \mid (EA_3 \mid a$

$Z_1 \rightarrow ^*FZ_1 \mid ^*F$

$F \rightarrow (EA_3 \mid a$

GNF, Greibach Normal Form-Example 4

Productions are

$E \rightarrow EA_1T \mid TA_2F \mid (EA_3 \mid a$

$T \rightarrow (EA_3Z_1 \mid aZ_1 \mid (EA_3 \mid a$

$Z_1 \rightarrow *FZ_1 \mid *F$

$F \rightarrow (EA_3 \mid a$

For Production $E \rightarrow TA_2F$, Substitute the value of T

Replace $E \rightarrow TA_2F$ by

$E \rightarrow (EA_3Z_1A_2F \mid aZ_1A_2F \mid (EA_3A_2F \mid aA_2F$

so Replace $E \rightarrow EA_1T \mid TA_2F \mid (EA_3 \mid a$ by

$E \rightarrow EA_1T \mid (EA_3Z_1A_2F \mid aZ_1A_2F \mid (EA_3A_2F \mid aA_2F \mid (EA_3 \mid a$

Productions are

$E \rightarrow EA_1T \mid (EA_3Z_1A_2F \mid aZ_1A_2F \mid (EA_3A_2F \mid aA_2F \mid (EA_3 \mid a$

$T \rightarrow (EA_3Z_1 \mid aZ_1 \mid (EA_3 \mid a$

$Z_1 \rightarrow *FZ_1 \mid *F$

$F \rightarrow (EA_3 \mid a$

All productions of E are in GNF except $E \rightarrow EA_1T$

GNF, Greibach Normal Form-Example 4

Productions are

$E \rightarrow EA_1T \mid (EA_3Z_1A_2F \mid aZ_1A_2F \mid (EA_3A_2F \mid aA_2F \mid (EA_3 \mid a$

$T \rightarrow (EA_3Z_1 \mid aZ_1 \mid (EA_3 \mid a$

$Z_1 \rightarrow *FZ_1 \mid *F$

$F \rightarrow (EA_3 \mid a$

All productions of E are in GNF except $E \rightarrow EA_1T$

Removing Left recursion for $E \rightarrow EA_1T$

Replace $E \rightarrow EA_1T \mid (EA_3Z_1A_2F \mid aZ_1A_2F \mid (EA_3A_2F \mid aA_2F \mid (EA_3 \mid a$ by

$E \rightarrow (EA_3Z_1A_2FZ_2 \mid aZ_1A_2FZ_2 \mid (EA_3A_2FZ_2 \mid aA_2FZ_2 \mid (EA_3Z_2 \mid aZ_2 \mid$
 $(EA_3Z_1A_2F \mid aZ_1A_2F \mid (EA_3A_2F \mid aA_2F \mid (EA_3 \mid a \mid$

$Z_2 \rightarrow A_1TZ_2 \mid A_1T$

Substituting + for A_1

$Z_2 \rightarrow +TZ_2 \mid +T$

Resulting grammar is-

$E \rightarrow (EA_3Z_1A_2FZ_2 \mid aZ_1A_2FZ_2 \mid (EA_3A_2FZ_2 \mid aA_2FZ_2 \mid (EA_3Z_2 \mid aZ_2 \mid$
 $(EA_3Z_1A_2F \mid aZ_1A_2F \mid (EA_3A_2F \mid aA_2F \mid (EA_3 \mid a \mid$

$Z_2 \rightarrow +TZ_2 \mid +T$

$T \rightarrow (EA_3Z_1 \mid aZ_1 \mid (EA_3 \mid a$

$Z_1 \rightarrow *FZ_1 \mid *F$

$F \rightarrow (EA_3 \mid a$